various attempts at defining memory

src/Memory.v
@@ -19,10 +19,10 @@ Section Memory.
     writeMem: M -> word w -> word w -> option M;
 
     readMem_succeeds: forall (m: M) (a: word w),
-      isReadableAddr m a -> exists v, readMem m a = Some v;
+      isReadableAddr m a -> exists v, readMem m a = Some v; (* TODO should be <-> *)
 
     writeMem_succeeds: forall (m: M) (a v: word w),
-      isWriteableAddr m a -> exists m', writeMem m a v = Some m';
+      isWriteableAddr m a -> exists m', writeMem m a v = Some m'; (* TODO should be <-> *)
 
     writeMem_preserves_isReadableAddr: forall (m: M) (a v: word w),
       match writeMem m a v with
@@ -46,24 +46,28 @@ Section Memory.
       forall b, b <> a -> readMem m' b = readMem m b;
   }.
 
+  Definition TODO{T: Type}: T. Admitted.
+
   (* TODO divide every address by 4? *)
   Instance ListIsMemory: Memory (list (word w)) := {|
-    isReadableAddr := fun m a => wordToNat a < length m;
-    isWriteableAddr := fun m a => wordToNat a < length m;
-    readMem := fun m a => nth_error m (wordToNat a);
-    writeMem := fun m a v => listUpdate_error m (wordToNat a) v
+    isReadableAddr := fun m a => wmod a $4 = $0 /\ wordToNat a / 4 < length m;
+    isWriteableAddr := fun m a => wmod a $4 = $0 /\ wordToNat a / 4 < length m;
+    readMem := fun m a => nth_error m (wordToNat a / 4);
+    writeMem := fun m a v => listUpdate_error m (wordToNat a / 4) v
   |}.
   all: intros.
-  - apply nth_error_Some in H. destruct (nth_error m # (a)); [eauto|contradiction].
-  - unfold listUpdate_error. destruct_one_match; [eauto|contradiction].
-  - unfold listUpdate_error. destruct (dec (# (a) < length m)); [|trivial].
+  - destruct H. apply nth_error_Some in H0. destruct (nth_error m (# a / 4)); [eauto|contradiction].
+  - destruct H. unfold listUpdate_error. destruct_one_match; [eauto|contradiction].
+  - unfold listUpdate_error. destruct (dec ((# a / 4) < length m)); [|trivial].
     rewrite listUpdate_length by assumption.
     reflexivity.
   - destruct_one_match; [|trivial].
     apply listUpdate_error_length in E. rewrite E. reflexivity.
   - eauto using nth_error_listUpdate_error_same.
   - eapply nth_error_listUpdate_error_diff; [eassumption|].
-    apply wordToNat_neq_inj. assumption.
+    (* TODO doesn't hold 
+    apply wordToNat_neq_inj. assumption. *)
+    apply TODO.
   Defined.
 
     (*
