src/Memory3.v
@@ -1,0 +1,23 @@
+Require Import Coq.Lists.List.
+Import ListNotations.
+Require Import Coq.omega.Omega.
+Require Import bbv.Word.
+Require Import compiler.Decidable.
+Require Import compiler.Tactics.
+Require Import compiler.ListLib.
+
+
+Section Memory.
+
+  Variable w: nat. (* bit width of addresses, registers, and sizes ("size_t" in C), XLEN in RISC-V *)
+
+  Class Memory(m: Type) := mkMemory {
+    (* we don't use these load/store/Byte/Half/Word/Double, but they could be added here *)
+
+    (* we only use these two, which are on 32 or 64 bits depending on XLEN: *)
+    load_size_t: m -> word w -> word w;
+    store_size_t: m -> word w -> word w -> m;
+  }.
+
+End Memory.
+
